Add if-then-else

src/e.lean
@@ -7,6 +7,7 @@ inductive exp: Type
 | succ: exp -> exp
 | true: exp
 | false: exp
+| if_: exp -> exp -> exp -> exp
 
 inductive typ: Type
 | nat: typ
@@ -17,6 +18,12 @@ inductive has_typ: exp -> typ -> Prop
 | succ (e: exp): has_typ e typ.nat -> has_typ (exp.succ e) typ.nat
 | true: has_typ exp.true typ.bool
 | false: has_typ exp.false typ.bool
+| if_
+    (cond: exp) (yes: exp) (no: exp) (t: typ):
+    has_typ cond typ.bool ->
+    has_typ yes t ->
+    has_typ no t ->
+    has_typ (exp.if_ cond yes no) t
 
 inductive val: exp -> Prop
 | zero: val exp.zero
@@ -26,6 +33,16 @@ inductive val: exp -> Prop
 
 inductive steps: exp -> exp -> Prop
 | succ (e: exp) (e': exp): steps e e' -> steps (exp.succ e) (exp.succ e')
+| if_cond
+    (cond: exp) (cond': exp) (yes: exp) (no: exp):
+    steps cond cond' ->
+    steps (exp.if_ cond yes no) (exp.if_ cond' yes no)
+| if_yes
+    (yes: exp) (no: exp):
+    steps (exp.if_ exp.true yes no) yes
+| if_no
+    (yes: exp) (no: exp):
+    steps (exp.if_ exp.false yes no) no
 
 -- helper theorems
 
@@ -38,6 +55,47 @@ begin
   split,
   exact typing_a,
   refl,
+end
+
+theorem inversion_if_cond
+  (cond: exp) (yes: exp) (no: exp) (t: typ)
+  (typing: has_typ (exp.if_ cond yes no) t)
+  : has_typ cond typ.bool :=
+begin
+  cases typing,
+  exact typing_a,
+end
+
+theorem inversion_if_yes
+  (cond: exp) (yes: exp) (no: exp) (t: typ)
+  (typing: has_typ (exp.if_ cond yes no) t)
+  : has_typ yes t :=
+begin
+  cases typing,
+  exact typing_a_1,
+end
+
+theorem inversion_if_no
+  (cond: exp) (yes: exp) (no: exp) (t: typ)
+  (typing: has_typ (exp.if_ cond yes no) t)
+  : has_typ no t :=
+begin
+  cases typing,
+  exact typing_a_2,
+end
+
+theorem bool_canonical_forms
+  (e: exp)
+  (typing: has_typ e typ.bool)
+  (value: val e)
+  : e = exp.true ∨ e = exp.false :=
+begin
+  cases typing,
+  left,
+  refl,
+  right,
+  refl,
+  cases value,
 end
 
 -- preservation
@@ -54,6 +112,13 @@ begin
   rewrite inv.right at *,
   apply has_typ.succ stepping_e',
   exact stepping_ih typ.nat left,
+  let inv := inversion_if_cond stepping_cond stepping_yes stepping_no t typing,
+  apply has_typ.if_ stepping_cond' stepping_yes stepping_no t,
+  exact stepping_ih typ.bool inv,
+  exact inversion_if_yes stepping_cond stepping_yes stepping_no t typing,
+  exact inversion_if_no stepping_cond stepping_yes stepping_no t typing,
+  exact inversion_if_yes exp.true stepping_yes stepping_no t typing,
+  exact inversion_if_no exp.false stepping_yes stepping_no t typing,
 end
 
 -- progress
@@ -77,4 +142,16 @@ begin
   exact val.true,
   left,
   exact val.false,
+  right,
+  cases typing_ih_a,
+  cases bool_canonical_forms typing_cond typing_a typing_ih_a,
+  existsi typing_yes,
+  rewrite h,
+  exact steps.if_yes typing_yes typing_no,
+  existsi typing_no,
+  rewrite h,
+  exact steps.if_no typing_yes typing_no,
+  cases typing_ih_a,
+  existsi (exp.if_ typing_ih_a_w typing_yes typing_no),
+  exact steps.if_cond typing_cond typing_ih_a_w typing_yes typing_no typing_ih_a_h,
 end
